Add support for a set of initially available capabilities
This normally shouldn't be necessary, as the ISA spec should only use
capabilities that have been directly read from registers or memory, but
allowing an initially available set of capabilities can be useful in
some corner cases.  For example, the Morello ASL spec contains a few cases
of UNKNOWN capabilities that can have arbitrary, nondeterministically
chosen values, only constrained by the prose spec to not increase the
capability rights available to software.  With this patch, we can model
these as capabilities chosen from an arbitrary but fixed subset of the
capabilities reachable from the initial state in the given context.

The monotonicity theorem still holds with the additional assumption that
these initial capabilities are indeed reachable in the initial state.

model/Recognising_Automata.thy
@@ -33,6 +33,9 @@ lemma trace_enabled_append_iff: "trace_enabled s (t @ t') \<longleftrightarrow> 
 lemma accepts_from_append_iff: "accepts_from s (t @ t') \<longleftrightarrow> trace_enabled s t \<and> accepts_from (run s t) t'"
   by (auto simp: accepts_from_def trace_enabled_append_iff)
 
+lemma accepts_from_Nil[simp]: "accepts_from s [] \<longleftrightarrow> final s"
+  by (auto simp: accepts_from_def)
+
 lemma accepts_from_Cons[simp]: "accepts_from s (e # t) \<longleftrightarrow> enabled s e \<and> accepts_from (step s e) t"
   by (auto simp: accepts_from_def)
 
@@ -272,8 +275,11 @@ record ('cap, 'regval) axiom_state =
 definition accessed_caps where
   "accessed_caps use_mem_caps s \<equiv> accessed_reg_caps s \<union> (if use_mem_caps then accessed_mem_caps s else {})"
 
-locale Cap_Axiom_Automaton = Capability_ISA CC ISA
-  for CC :: "'cap Capability_class" and ISA :: "('cap, 'regval, 'instr, 'e) isa" +
+abbreviation (in Capability_ISA) "tagged_initial_caps \<equiv> {c \<in> initial_caps. is_tagged_method CC c}"
+
+locale Cap_Axiom_Automaton = Capability_ISA CC ISA initial_caps
+  for CC :: "'cap Capability_class" and ISA :: "('cap, 'regval, 'instr, 'e) isa"
+    and initial_caps :: "'cap set" +
   fixes enabled :: "('cap, 'regval) axiom_state \<Rightarrow> 'regval event \<Rightarrow> bool"
     and use_mem_caps :: bool
 begin
@@ -607,16 +613,33 @@ lemma non_mem_exp_foreachM:
   using assms
   by (induction xs vars body rule: foreachM.induct) (auto intro: non_cap_expI[THEN non_cap_exp_non_mem_exp])
 
-lemma non_cap_exp_choose_bool[non_cap_expI]:
-  "non_cap_exp (choose_bool desc)"
-  by (auto simp: choose_bool_def non_cap_exp_def elim: Traces_cases)
+lemma non_cap_exp_choose_regval[non_cap_expI]:
+  "non_cap_exp (choose_regval desc)"
+  by (auto simp: choose_regval_def non_cap_exp_def elim: Traces_cases)
 
-lemma non_cap_exp_undefined_bool[non_cap_expI]:
-  "non_cap_exp (undefined_bool ())"
-  by (auto simp: undefined_bool_def intro: non_cap_expI)
+lemma non_cap_exp_undefined_value[non_cap_expI]:
+  "non_cap_exp (choose_convert of_rv descr)"
+  unfolding choose_convert_def maybe_fail_def
+  by (auto simp: non_cap_exp_def elim: Traces_cases split: option.splits)
+
+lemma non_cap_exp_choose_bool[non_cap_expI]:
+  "non_cap_exp (choose_bool RV desc)"
+  by (auto simp: choose_bool_def intro: non_cap_expI)
+
+lemma non_cap_exp_choose_int[non_cap_expI]:
+  "non_cap_exp (choose_int RV msg)"
+  by (auto simp: choose_int_def intro: non_cap_expI)
+
+lemma non_cap_exp_choose_real[non_cap_expI]:
+  "non_cap_exp (choose_real RV msg)"
+  by (auto simp: choose_real_def intro: non_cap_expI)
+
+lemma non_cap_exp_choose_string[non_cap_expI]:
+  "non_cap_exp (choose_string RV msg)"
+  by (auto simp: choose_string_def intro: non_cap_expI)
 
 lemma non_cap_exp_bool_of_bitU_nondet[non_cap_expI]:
-  "non_cap_exp (bool_of_bitU_nondet b)"
+  "non_cap_exp (bool_of_bitU_nondet RV b)"
   unfolding bool_of_bitU_nondet_def
   by (cases b) (auto intro: non_cap_expI)
 
@@ -634,11 +657,11 @@ lemma non_cap_exp_bool_of_bitU_fail[non_cap_expI]:
   by (cases b) (auto intro: non_cap_expI)
 
 lemma non_cap_exp_bools_of_bits_nondet[non_cap_expI]:
-  "non_cap_exp (bools_of_bits_nondet bits)"
+  "non_cap_exp (bools_of_bits_nondet RV bits)"
   by (auto simp: bools_of_bits_nondet_def intro: non_cap_expI)
 
 lemma non_cap_exp_of_bits_nondet[non_cap_expI]:
-  "non_cap_exp (of_bits_nondet BC bits)"
+  "non_cap_exp (of_bits_nondet BC RV bits)"
   by (auto simp: of_bits_nondet_def intro: non_cap_expI)
 
 lemma non_cap_exp_of_bits_fail[non_cap_expI]:
@@ -646,7 +669,7 @@ lemma non_cap_exp_of_bits_fail[non_cap_expI]:
   by (auto simp: of_bits_fail_def intro: non_cap_expI)
 
 lemma non_cap_exp_mword_nondet[non_cap_expI]:
-  "non_cap_exp (mword_nondet ())"
+  "non_cap_exp (mword_nondet RV ())"
   by (auto simp add: mword_nondet_def intro: non_cap_expI simp del: repeat.simps)
 
 lemma non_cap_exp_genlistM:
@@ -656,7 +679,7 @@ lemma non_cap_exp_genlistM:
   by (auto simp: genlistM_def intro!: non_cap_expI)
 
 lemma non_cap_exp_choose_bools[non_cap_expI]:
-  "non_cap_exp (choose_bools desc n)"
+  "non_cap_exp (choose_bools RV desc n)"
   by (auto simp: choose_bools_def intro: non_cap_expI non_cap_exp_genlistM)
 
 lemma non_cap_exp_exit[non_cap_expI]:
@@ -665,12 +688,8 @@ lemma non_cap_exp_exit[non_cap_expI]:
   by (rule non_cap_exp_Fail)
 
 lemma non_cap_exp_chooseM[non_cap_expI]:
-  "non_cap_exp (chooseM desc xs)"
-  by (auto simp: chooseM_def intro!: non_cap_expI split: option.splits)
-
-lemma non_cap_exp_internal_pick[non_cap_expI]:
-  "non_cap_exp (internal_pick xs)"
-  by (auto simp: internal_pick_def intro!: non_cap_expI)
+  "non_cap_exp (choose_from_list RV desc xs)"
+  by (auto simp: choose_from_list_def intro!: non_cap_expI split: option.splits)
 
 lemma non_cap_exp_and_boolM[intro!]:
   "non_cap_exp (and_boolM m1 m2)" if "non_cap_exp m1" and "non_cap_exp m2"
@@ -905,10 +924,11 @@ method accessible_regsI uses simp assms =
      simp: simp assms: assms)
 
 definition derivable_caps :: "('cap, 'regval) axiom_state \<Rightarrow> 'cap set" where
-  "derivable_caps s \<equiv> {c. is_tagged_method CC c \<longrightarrow> c \<in> derivable (accessed_caps use_mem_caps s)}"
+  "derivable_caps s \<equiv>
+     {c. is_tagged_method CC c \<longrightarrow> c \<in> derivable (initial_caps \<union> accessed_caps use_mem_caps s)}"
 
 definition derivable_mem_caps where
-  "derivable_mem_caps s = {c. is_tagged_method CC c \<longrightarrow> c \<in> derivable (accessed_mem_caps s)}"
+  "derivable_mem_caps s = {c. is_tagged_method CC c \<longrightarrow> c \<in> derivable (initial_caps \<union> accessed_mem_caps s)}"
 
 definition accessed_mem_caps_of_trace where
   "accessed_mem_caps_of_trace t = (\<Union>e \<in> set t. accessed_mem_caps_of_ev e)"
@@ -963,9 +983,15 @@ lemma derivable_mem_caps_derivable_caps:
   assumes "c \<in> derivable_mem_caps s"
     and "use_mem_caps"
   shows "c \<in> derivable_caps s"
-  using assms(1)
-  using derivable_mono[of "accessed_mem_caps s" "accessed_reg_caps s \<union> accessed_mem_caps s"]
-  by (auto simp: derivable_mem_caps_def derivable_caps_def accessed_caps_def intro: assms(2))
+proof -
+  have "initial_caps \<union> accessed_mem_caps s \<subseteq> initial_caps \<union> accessed_caps use_mem_caps s"
+    using assms(2)
+    by (auto simp: accessed_caps_def)
+  from derivable_mono[OF this]
+  show ?thesis
+    using assms(1)
+    by (auto simp: derivable_mem_caps_def derivable_caps_def)
+qed
 
 named_theorems derivable_capsE
 named_theorems derivable_capsI
@@ -986,7 +1012,7 @@ lemma accessed_caps_run_mono:
 
 lemma derivable_caps_run_mono:
   "derivable_caps s \<subseteq> derivable_caps (run s t)"
-  using derivable_mono[OF accessed_caps_run_mono]
+  using derivable_mono[OF accessed_caps_run_mono[THEN Un_mono[OF subset_refl]]]
   by (auto simp: derivable_caps_def)
 
 lemma derivable_caps_run_imp:
@@ -1122,8 +1148,9 @@ lemma recognises_store_cap_mem_axiom:
 
 end*)
 
-locale Write_Cap_Automaton = Capability_ISA CC ISA
-  for CC :: "'cap Capability_class" and ISA :: "('cap, 'regval, 'instr, 'e) isa" +
+locale Write_Cap_Automaton = Capability_ISA CC ISA initial_caps
+  for CC :: "'cap Capability_class" and ISA :: "('cap, 'regval, 'instr, 'e) isa"
+    and initial_caps :: "'cap set" +
   fixes ex_traces :: bool and use_mem_caps :: bool
     and invoked_caps :: "'cap set" and invoked_indirect_caps :: "'cap set"
 begin
@@ -1135,54 +1162,54 @@ fun enabled :: "('cap, 'regval) axiom_state \<Rightarrow> 'regval event \<Righta
      (r \<in> write_privileged_regs ISA \<longrightarrow> (system_reg_access s \<or> r \<in> write_exception_regs ISA \<and> ex_traces)) \<and>
      (\<forall>c. (c \<in> caps_of_regval ISA v \<and> is_tagged_method CC c)
          \<longrightarrow>
-         (c \<in> derivable (accessed_caps (\<not>invokes_indirect_caps \<and> use_mem_caps) s) \<or>
+         (c \<in> derivable (initial_caps \<union> accessed_caps (\<not>invokes_indirect_caps \<and> use_mem_caps) s) \<or>
           (c \<in> exception_targets ISA (read_from_KCC s) \<and> ex_traces \<and> r \<in> PCC ISA) \<or>
-          (\<exists>cs. c \<in> invoked_caps \<and> cs \<in> derivable (accessed_caps (\<not>invokes_indirect_caps \<and> use_mem_caps) s) \<and>
+          (\<exists>cs. c \<in> invoked_caps \<and> cs \<in> derivable (initial_caps \<union> accessed_caps (\<not>invokes_indirect_caps \<and> use_mem_caps) s) \<and>
                 is_sentry_method CC cs \<and> is_sealed_method CC cs \<and>
                 leq_cap CC c (unseal_method CC cs) \<and> r \<in> PCC ISA) \<or>
-          (\<exists>cs. c \<in> invoked_indirect_caps \<and> cs \<in> derivable (accessed_reg_caps s) \<and>
+          (\<exists>cs. c \<in> invoked_indirect_caps \<and> cs \<in> derivable (initial_caps \<union> accessed_reg_caps s) \<and>
                 is_indirect_sentry_method CC cs \<and> is_sealed_method CC cs \<and>
                 leq_cap CC c (unseal_method CC cs) \<and> r \<in> IDC ISA) \<or>
           (\<exists>cc cd. c \<in> invoked_caps \<and> invokable CC cc cd \<and>
-                   cc \<in> derivable (accessed_caps (\<not>invokes_indirect_caps \<and> use_mem_caps) s) \<and>
-                   cd \<in> derivable (accessed_caps (\<not>invokes_indirect_caps \<and> use_mem_caps) s) \<and>
+                   cc \<in> derivable (initial_caps \<union> accessed_caps (\<not>invokes_indirect_caps \<and> use_mem_caps) s) \<and>
+                   cd \<in> derivable (initial_caps \<union> accessed_caps (\<not>invokes_indirect_caps \<and> use_mem_caps) s) \<and>
                    (r \<in> PCC ISA \<and> leq_cap CC c (unseal_method CC cc) \<or>
                     r \<in> IDC ISA \<and> leq_cap CC c (unseal_method CC cd))) \<or>
           (\<exists>c'. c \<in> invoked_caps \<and>
-                c' \<in> derivable (accessed_mem_caps s) \<and>
+                c' \<in> derivable (initial_caps \<union> accessed_mem_caps s) \<and>
                 ((leq_cap CC c (unseal_method CC c') \<and> is_sealed_method CC c' \<and> is_sentry_method CC c' \<and> r \<in> PCC ISA) \<or>
                  (leq_cap CC c c' \<and> r \<in> PCC ISA \<union> IDC ISA)))))"
 | "enabled s (E_read_reg r v) = (r \<in> read_privileged_regs ISA \<longrightarrow> (system_reg_access s \<or> r \<in> read_exception_regs ISA \<and> ex_traces))"
 | "enabled s (E_write_memt _ addr sz bytes tag _) =
-     (\<forall>c.  cap_of_mem_bytes_method CC bytes tag = Some c \<and> is_tagged_method CC c \<longrightarrow> c \<in> derivable (accessed_caps (\<not>invokes_indirect_caps \<and> use_mem_caps) s))"
+     (\<forall>c.  cap_of_mem_bytes_method CC bytes tag = Some c \<and> is_tagged_method CC c \<longrightarrow> c \<in> derivable (initial_caps \<union> accessed_caps (\<not>invokes_indirect_caps \<and> use_mem_caps) s))"
 | "enabled s _ = True"
 
 lemma enabled_E_write_reg_cases:
   assumes "enabled s (E_write_reg r v)"
     and "c \<in> caps_of_regval ISA v"
     and "is_tagged_method CC c"
-  obtains (Derivable) "c \<in> derivable (accessed_caps (\<not>invokes_indirect_caps \<and> use_mem_caps) s)"
+  obtains (Derivable) "c \<in> derivable (initial_caps \<union> accessed_caps (\<not>invokes_indirect_caps \<and> use_mem_caps) s)"
   | (KCC) "c \<in> exception_targets ISA (read_from_KCC s)" and "ex_traces" and
-      "r \<in> PCC ISA" and "c \<notin> derivable (accessed_caps (\<not>invokes_indirect_caps \<and> use_mem_caps) s)"
-  | (Sentry) cs where "c \<in> invoked_caps" and "cs \<in> derivable (accessed_caps (\<not>invokes_indirect_caps \<and> use_mem_caps) s)" and
+      "r \<in> PCC ISA" and "c \<notin> derivable (initial_caps \<union> accessed_caps (\<not>invokes_indirect_caps \<and> use_mem_caps) s)"
+  | (Sentry) cs where "c \<in> invoked_caps" and "cs \<in> derivable (initial_caps \<union> accessed_caps (\<not>invokes_indirect_caps \<and> use_mem_caps) s)" and
       "is_sentry_method CC cs" and "is_sealed_method CC cs" and
       "leq_cap CC c (unseal_method CC cs)" and "r \<in> PCC ISA"
-  | (SentryIndirect) cs where "c \<in> invoked_indirect_caps" and "cs \<in> derivable (accessed_reg_caps s)" and
+  | (SentryIndirect) cs where "c \<in> invoked_indirect_caps" and "cs \<in> derivable (initial_caps \<union> accessed_reg_caps s)" and
       "is_indirect_sentry_method CC cs" and "is_sealed_method CC cs" and
       "leq_cap CC c (unseal_method CC cs)" and "r \<in> IDC ISA"
   | (CCall) cc cd where "c \<in> invoked_caps" and "invokable CC cc cd" and
-      "cc \<in> derivable (accessed_caps (\<not>invokes_indirect_caps \<and> use_mem_caps) s)" and
-      "cd \<in> derivable (accessed_caps (\<not>invokes_indirect_caps \<and> use_mem_caps) s)" and
+      "cc \<in> derivable (initial_caps \<union> accessed_caps (\<not>invokes_indirect_caps \<and> use_mem_caps) s)" and
+      "cd \<in> derivable (initial_caps \<union> accessed_caps (\<not>invokes_indirect_caps \<and> use_mem_caps) s)" and
       "r \<in> PCC ISA \<and> leq_cap CC c (unseal_method CC cc) \<or> r \<in> IDC ISA \<and> leq_cap CC c (unseal_method CC cd)" and
-      "c \<notin> derivable (accessed_caps (\<not>invokes_indirect_caps \<and> use_mem_caps) s)"
+      "c \<notin> derivable (initial_caps \<union> accessed_caps (\<not>invokes_indirect_caps \<and> use_mem_caps) s)"
   | (Indirect) c' where "c \<in> invoked_caps" and
-      "c' \<in> derivable (accessed_mem_caps s)"
+      "c' \<in> derivable (initial_caps \<union> accessed_mem_caps s)"
       "(leq_cap CC c (unseal_method CC c') \<and> is_sealed_method CC c' \<and> is_sentry_method CC c' \<and> r \<in> PCC ISA) \<or>
        (leq_cap CC c c' \<and> r \<in> PCC ISA \<union> IDC ISA)"
   using assms
-  by (cases "c \<in> derivable (accessed_caps (\<not>invokes_indirect_caps \<and> use_mem_caps) s)"; auto; fastforce)
+  by (cases "c \<in> derivable (initial_caps \<union> accessed_caps (\<not>invokes_indirect_caps \<and> use_mem_caps) s)"; auto; fastforce)
 
-sublocale Cap_Axiom_Automaton CC ISA enabled "invoked_indirect_caps = {} \<and> use_mem_caps" ..
+sublocale Cap_Axiom_Automaton CC ISA initial_caps enabled "invoked_indirect_caps = {} \<and> use_mem_caps" ..
 
 lemma non_cap_event_enabledI:
   assumes "non_cap_event e"
@@ -1221,8 +1248,8 @@ lemma index_eq_some': "(index l n = Some x) = (n < length l \<and> l ! n = x)"
 
 lemma recognises_store_cap_reg_read_reg_axioms:
   assumes t: "accepts t"
-  shows "store_cap_reg_axiom CC ISA ex_traces use_mem_caps invoked_caps invoked_indirect_caps t"
-    and "store_cap_mem_axiom CC ISA use_mem_caps invoked_indirect_caps t"
+  shows "store_cap_reg_axiom CC ISA ex_traces initial_caps use_mem_caps invoked_caps invoked_indirect_caps t"
+    and "store_cap_mem_axiom CC ISA initial_caps use_mem_caps invoked_indirect_caps t"
     and "read_reg_axiom CC ISA ex_traces t"
     and "write_reg_axiom CC ISA ex_traces t"
 proof -
@@ -1230,7 +1257,7 @@ proof -
     using assms (*read_from_KCC_run_take_eq[of "length t" t]*)
     unfolding accepts_from_iff_all_enabled_final read_reg_axiom_def write_reg_axiom_def
     by (auto elim!: enabled.elims)
-  show "store_cap_reg_axiom CC ISA ex_traces use_mem_caps invoked_caps invoked_indirect_caps t"
+  show "store_cap_reg_axiom CC ISA ex_traces initial_caps use_mem_caps invoked_caps invoked_indirect_caps t"
   proof (unfold store_cap_reg_axiom_def, intro allI impI, goal_cases Idx)
     case (Idx i c r)
     then show ?case
@@ -1278,7 +1305,7 @@ proof -
       qed
     qed auto
   qed
-  show "store_cap_mem_axiom CC ISA use_mem_caps invoked_indirect_caps t"
+  show "store_cap_mem_axiom CC ISA initial_caps use_mem_caps invoked_indirect_caps t"
     using assms
     unfolding accepts_from_iff_all_enabled_final store_cap_mem_axiom_def
     by (auto simp: cap_derivable_iff_derivable writes_mem_cap_Some_iff)
@@ -1287,8 +1314,10 @@ qed
 end
 
 locale Cap_Axiom_Assm_Automaton =
-  Capability_Invariant_ISA CC ISA cap_invariant + Cap_Axiom_Automaton CC ISA enabled use_mem_caps
+  Capability_Invariant_ISA CC ISA initial_caps cap_invariant +
+  Cap_Axiom_Automaton CC ISA initial_caps enabled use_mem_caps
   for CC :: "'cap Capability_class" and ISA :: "('cap, 'regval, 'instr, 'e) isa"
+    and initial_caps :: "'cap set"
     and cap_invariant :: "'cap \<Rightarrow> bool"
     and enabled :: "('cap, 'regval) axiom_state \<Rightarrow> 'regval event \<Rightarrow> bool"
     and use_mem_caps :: bool +
@@ -1310,7 +1339,8 @@ lemma trace_assms_Cons[iff]: "trace_assms (e # t) \<longleftrightarrow> ev_assms
   by (auto simp: trace_assms_def)
 
 definition accessed_caps_invariant :: "('cap, 'regval) axiom_state \<Rightarrow> bool" where
-  "accessed_caps_invariant s \<equiv> (\<forall>c \<in> accessed_caps use_mem_caps s. is_tagged_method CC c \<longrightarrow> cap_invariant c)"
+  "accessed_caps_invariant s \<equiv>
+     (\<forall>c \<in> initial_caps \<union> accessed_caps use_mem_caps s. is_tagged_method CC c \<longrightarrow> cap_invariant c)"
 
 definition accessed_caps_trace_invariant :: "('cap, 'regval) axiom_state \<Rightarrow> 'regval event list \<Rightarrow> bool" where
   "accessed_caps_trace_invariant s t \<equiv> (\<forall>i \<le> length t. accessed_caps_invariant (run s (take i t)))"
@@ -1387,6 +1417,7 @@ lemma pre_inv_trace_assms_append_cases:
 lemma pre_inv_trace_assms_initialI:
   assumes "available_caps_invariant use_mem_caps t n" and "trace_assms (take n t)"
     and "n \<le> length t"
+    and "n = 0 \<longrightarrow> (\<forall>c \<in> initial_caps. is_tagged_method CC c \<longrightarrow> cap_invariant c)"
   shows "pre_inv_trace_assms initial (take n t)"
   using assms
   unfolding available_caps_invariant_def pre_inv_trace_assms_def accessed_caps_trace_invariant_def accessed_caps_invariant_def
@@ -1474,7 +1505,7 @@ lemma traces_enabled_acceptsI:
     and "available_caps_invariant use_mem_caps t n" and "trace_assms (take n t)" and "n \<le> length t"
   shows "accepts (take n t)"
   using assms
-  by (intro traces_enabled_accepts_from_takeI pre_inv_trace_assms_initialI)
+  by (cases n; auto intro: traces_enabled_accepts_from_takeI pre_inv_trace_assms_initialI)
 
 lemma traces_enabled_accepts_fromI:
   assumes "hasTrace t m" and "traces_enabled m s" and "hasException t m \<or> hasFailure t m \<longrightarrow> ex_traces"
@@ -2179,9 +2210,11 @@ lemma if_derivable_capsI[derivable_capsI]:
 
 end
 
-locale Cap_Axiom_Inv_Automaton = Cap_Axiom_Automaton CC ISA enabled use_mem_caps +
+locale Cap_Axiom_Inv_Automaton =
+  Cap_Axiom_Automaton CC ISA initial_caps enabled use_mem_caps +
   State_Invariant get_regval set_regval invariant inv_regs
   for CC :: "'cap Capability_class" and ISA :: "('cap, 'regval, 'instr, 'e) isa"
+    and initial_caps :: "'cap set"
     and enabled :: "('cap, 'regval) axiom_state \<Rightarrow> 'regval event \<Rightarrow> bool"
     and use_mem_caps :: bool
     and get_regval :: "string \<Rightarrow> 'regstate \<Rightarrow> 'regval option"
@@ -2550,9 +2583,10 @@ lemma if_derivable_capsI[derivable_capsI]:
 end
 
 locale Write_Cap_Assm_Automaton =
-  Capability_Invariant_ISA CC ISA cap_invariant +
-  Write_Cap_Automaton CC ISA ex_traces use_mem_caps invoked_caps invoked_indirect_caps
+  Capability_Invariant_ISA CC ISA initial_caps cap_invariant +
+  Write_Cap_Automaton CC ISA initial_caps ex_traces use_mem_caps invoked_caps invoked_indirect_caps
   for CC :: "'cap Capability_class" and ISA :: "('cap, 'regval, 'instr, 'e) isa"
+  and initial_caps :: "'cap set"
   and cap_invariant :: "'cap \<Rightarrow> bool"
   and ex_traces :: bool and use_mem_caps :: bool
   and invoked_caps :: "'cap set" and invoked_indirect_caps :: "'cap set" +
@@ -2632,8 +2666,8 @@ lemma traces_enabled_reg_axioms:
   assumes "traces_enabled m initial" and "hasTrace t m"
     and "pre_inv_trace_assms initial t"
     and "hasException t m \<or> hasFailure t m \<longrightarrow> ex_traces"
-  shows "store_cap_reg_axiom CC ISA ex_traces use_mem_caps invoked_caps invoked_indirect_caps t"
-    and "store_cap_mem_axiom CC ISA use_mem_caps invoked_indirect_caps t"
+  shows "store_cap_reg_axiom CC ISA ex_traces initial_caps use_mem_caps invoked_caps invoked_indirect_caps t"
+    and "store_cap_mem_axiom CC ISA initial_caps use_mem_caps invoked_indirect_caps t"
     and "read_reg_axiom CC ISA ex_traces t"
   using assms
   by (intro recognises_store_cap_reg_read_reg_axioms;
@@ -2643,9 +2677,10 @@ lemma traces_enabled_reg_axioms:
 end
 
 locale Write_Cap_Inv_Automaton =
-  Write_Cap_Automaton CC ISA ex_traces use_mem_caps invoked_caps invoked_indirect_caps +
+  Write_Cap_Automaton CC ISA initial_caps ex_traces use_mem_caps invoked_caps invoked_indirect_caps +
   State_Invariant get_regval set_regval invariant inv_regs
   for CC :: "'cap Capability_class" and ISA :: "('cap, 'regval, 'instr, 'e) isa"
+    and initial_caps :: "'cap set"
     and ex_traces :: bool and use_mem_caps :: bool
     and invoked_caps :: "'cap set" and invoked_indirect_caps :: "'cap set"
     and get_regval :: "string \<Rightarrow> 'regstate \<Rightarrow> 'regval option"
@@ -2698,8 +2733,8 @@ lemma traces_enabled_reg_axioms:
   assumes "traces_enabled m initial regs" and "hasTrace t m"
     and "reads_regs_from inv_regs t regs" and "invariant regs"
     and "hasException t m \<or> hasFailure t m \<longrightarrow> ex_traces"
-  shows "store_cap_reg_axiom CC ISA ex_traces use_mem_caps invoked_caps invoked_indirect_caps t"
-    and "store_cap_mem_axiom CC ISA use_mem_caps invoked_indirect_caps t"
+  shows "store_cap_reg_axiom CC ISA ex_traces initial_caps use_mem_caps invoked_caps invoked_indirect_caps t"
+    and "store_cap_mem_axiom CC ISA initial_caps use_mem_caps invoked_indirect_caps t"
     and "read_reg_axiom CC ISA ex_traces t"
   using assms
   by (intro recognises_store_cap_reg_read_reg_axioms;
@@ -2708,8 +2743,9 @@ lemma traces_enabled_reg_axioms:
 
 end
 
-locale Capability_ISA_Fixed_Translation = Capability_ISA CC ISA
-  for CC :: "'cap Capability_class" and ISA :: "('cap, 'regval, 'instr, 'e) isa" +
+locale Capability_ISA_Fixed_Translation = Capability_ISA CC ISA initial_caps
+  for CC :: "'cap Capability_class" and ISA :: "('cap, 'regval, 'instr, 'e) isa"
+    and initial_caps :: "'cap set" +
   fixes translation_assms :: "'regval event \<Rightarrow> bool"
   assumes fixed_translation: "\<And>i t addr load. \<forall>e \<in> set t. translation_assms e \<Longrightarrow> translate_address ISA addr load (take i t) = translate_address ISA addr load []"
 begin
@@ -2728,26 +2764,28 @@ abbreviation non_store_trace :: "'regval trace \<Rightarrow> bool" where
 
 lemma (in Cap_Axiom_Automaton) non_mem_trace_mem_axiomsI:
   assumes "non_mem_trace t"
-  shows "store_mem_axiom CC ISA use_mem_caps invoked_indirect_caps t"
+  shows "store_mem_axiom CC ISA initial_caps use_mem_caps invoked_indirect_caps t"
     and "store_tag_axiom CC ISA t"
-    and "load_mem_axiom CC ISA is_fetch use_mem_caps invoked_indirect_caps t"
+    and "load_mem_axiom CC ISA is_fetch initial_caps use_mem_caps invoked_indirect_caps t"
 proof -
   have i: "non_mem_event (t ! i)" if "i < length t" for i
     using assms that
     by (auto simp: non_mem_trace_def)
-  show "store_mem_axiom CC ISA use_mem_caps invoked_indirect_caps t"
+  show "store_mem_axiom CC ISA initial_caps use_mem_caps invoked_indirect_caps t"
     using i
     by (fastforce simp: store_mem_axiom_def writes_mem_val_at_idx_def bind_eq_Some_conv elim!: writes_mem_val.elims)
   show "store_tag_axiom CC ISA t"
     using i
     by (fastforce simp: store_tag_axiom_def writes_mem_val_at_idx_def bind_eq_Some_conv elim!: writes_mem_val.elims)
-  show "load_mem_axiom CC ISA is_fetch use_mem_caps invoked_indirect_caps t"
+  show "load_mem_axiom CC ISA is_fetch initial_caps use_mem_caps invoked_indirect_caps t"
     using i
     by (fastforce simp: load_mem_axiom_def reads_mem_val_at_idx_def bind_eq_Some_conv elim!: reads_mem_val.elims)
 qed
 
-locale Mem_Automaton = Capability_ISA_Fixed_Translation where CC = CC and ISA = ISA
-  for CC :: "'cap Capability_class" and ISA :: "('cap, 'regval, 'instr, 'e) isa" +
+locale Mem_Automaton = Capability_ISA_Fixed_Translation CC ISA initial_caps translation_assms
+  for CC :: "'cap Capability_class" and ISA :: "('cap, 'regval, 'instr, 'e) isa"
+    and initial_caps :: "'cap set"
+    and translation_assms :: "'regval event \<Rightarrow> bool" +
   fixes is_fetch :: bool and use_mem_caps :: bool
     and invoked_indirect_caps :: "'cap set"
 begin
@@ -2782,7 +2820,7 @@ definition access_enabled :: "('cap, 'regval) axiom_state \<Rightarrow> acctype 
      ((tag \<noteq> B0 \<longrightarrow> address_tag_aligned ISA paddr \<and> sz = tag_granule ISA) \<and>
       (acctype = Fetch \<longrightarrow> tag = B0) \<and>
       (acctype = PTW \<or>
-       (\<exists>c' \<in> derivable (accessed_caps (invoked_indirect_caps = {} \<and> use_mem_caps) s).
+       (\<exists>c' \<in> derivable (initial_caps \<union> accessed_caps (invoked_indirect_caps = {} \<and> use_mem_caps) s).
           let is_cap = tag \<noteq> B0 in
           let is_local_cap = mem_val_is_local_cap CC ISA v tag \<and> tag = B1 in
           authorises_access c' acctype is_cap is_local_cap vaddr paddr sz)))"
@@ -2817,7 +2855,7 @@ sublocale Cap_Axiom_Automaton where enabled = enabled and use_mem_caps = "invoke
 
 lemma accepts_store_mem_axiom:
   assumes *: "translation_assms_trace t" and  **: "accepts t"
-  shows "store_mem_axiom CC ISA use_mem_caps invoked_indirect_caps t"
+  shows "store_mem_axiom CC ISA initial_caps use_mem_caps invoked_indirect_caps t"
   using accepts_from_nth_enabledI[OF **]
   unfolding store_mem_axiom_def
   unfolding writes_mem_val_at_idx_def cap_derivable_iff_derivable
@@ -2834,7 +2872,7 @@ lemma accepts_store_tag_axiom:
 
 lemma accepts_load_mem_axiom:
   assumes *: "translation_assms_trace t" and  **: "accepts t"
-  shows "load_mem_axiom CC ISA is_fetch use_mem_caps invoked_indirect_caps t"
+  shows "load_mem_axiom CC ISA is_fetch initial_caps use_mem_caps invoked_indirect_caps t"
   unfolding load_mem_axiom_def
   unfolding reads_mem_val_at_idx_def cap_derivable_iff_derivable
   unfolding translation_event_at_idx_def
@@ -2855,9 +2893,10 @@ lemma non_mem_trace_enabledI:
 end
 
 locale Mem_Assm_Automaton =
-  Capability_Invariant_ISA CC ISA cap_invariant +
-  Mem_Automaton translation_assms CC ISA is_fetch use_mem_caps invoked_indirect_caps
+  Capability_Invariant_ISA CC ISA initial_caps cap_invariant +
+  Mem_Automaton CC ISA initial_caps translation_assms is_fetch use_mem_caps invoked_indirect_caps
   for CC :: "'cap Capability_class" and ISA :: "('cap, 'regval, 'instr, 'e) isa"
+    and initial_caps :: "'cap set"
     and cap_invariant :: "'cap \<Rightarrow> bool"
     and translation_assms :: "'regval event \<Rightarrow> bool"
     and is_fetch :: bool and ex_traces :: bool and use_mem_caps :: bool
@@ -2895,9 +2934,9 @@ lemma traces_enabled_mem_axioms:
   assumes "traces_enabled m initial" and "hasTrace t m"
     and "pre_inv_trace_assms initial t"
     and "hasException t m \<or> hasFailure t m \<longrightarrow> ex_traces"
-  shows "store_mem_axiom CC ISA use_mem_caps invoked_indirect_caps t"
+  shows "store_mem_axiom CC ISA initial_caps use_mem_caps invoked_indirect_caps t"
     and "store_tag_axiom CC ISA t"
-    and "load_mem_axiom CC ISA is_fetch use_mem_caps invoked_indirect_caps t"
+    and "load_mem_axiom CC ISA is_fetch initial_caps use_mem_caps invoked_indirect_caps t"
   using assms
   by (intro accepts_store_mem_axiom accepts_store_tag_axiom accepts_load_mem_axiom
             traces_enabled_accepts_fromI;
@@ -2938,9 +2977,10 @@ lemma traces_enabled_read_memt:
 end
 
 locale Mem_Inv_Automaton =
-  Mem_Automaton translation_assms CC ISA is_fetch use_mem_caps invoked_indirect_caps +
+  Mem_Automaton CC ISA initial_caps translation_assms is_fetch use_mem_caps invoked_indirect_caps +
   State_Invariant get_regval set_regval invariant inv_regs
   for CC :: "'cap Capability_class" and ISA :: "('cap, 'regval, 'instr, 'e) isa"
+    and initial_caps :: "'cap set"
     and translation_assms :: "'regval event \<Rightarrow> bool"
     and is_fetch :: bool and ex_traces :: bool and use_mem_caps :: bool
     and invoked_indirect_caps :: "'cap set"
@@ -2977,9 +3017,9 @@ lemma traces_enabled_mem_axioms:
     and "reads_regs_from inv_regs t regs" and "invariant regs"
     and "hasException t m \<or> hasFailure t m \<longrightarrow> ex_traces"
     and "translation_assms_trace t"
-  shows "store_mem_axiom CC ISA use_mem_caps invoked_indirect_caps t"
+  shows "store_mem_axiom CC ISA initial_caps use_mem_caps invoked_indirect_caps t"
     and "store_tag_axiom CC ISA t"
-    and "load_mem_axiom CC ISA is_fetch use_mem_caps invoked_indirect_caps t"
+    and "load_mem_axiom CC ISA is_fetch initial_caps use_mem_caps invoked_indirect_caps t"
   using assms
   by (intro accepts_store_mem_axiom accepts_store_tag_axiom accepts_load_mem_axiom
             traces_enabled_accepts_fromI[where m = m and regs = regs];
